rewrite

reinvent/cat01.v
@@ -1,175 +1,279 @@
 Generalizable All Variables.
 Require Export Coq.Program.Basics Coq.Program.Tactics Coq.Setoids.Setoid Coq.Classes.Morphisms.
 
-(* Obligation Tactic := (try split); program_simpl; try now auto. *)
+Declare Scope setoid_scope.
+Open Scope setoid_scope.
 
-Module Setoid.
-  Structure Setoid : Type := {
-    setoid_carrier :> Type;
-    setoid_equal: setoid_carrier -> setoid_carrier -> Prop;
-    setoid_prf :> Equivalence setoid_equal
-  }.
-  #[global]
-  Existing Instance setoid_prf.
+Structure Setoid : Type := {
+  setoid_carrier:> Type;
+  setoid_equal: relation setoid_carrier;
+  setoid_prf:> Equivalence setoid_equal
+}.
+#[global]
+Existing Instance setoid_prf.
 
-  Notation "[ 'Setoid' 'by' P 'on' A ]" := (@Build_Setoid A P _).
-  Notation "[ 'Setoid' 'by' P ]" := [Setoid by P on _].
+Notation "[ 'Setoid' 'by' P 'on' A ]" := (@Build_Setoid A P _).
+Notation "[ 'Setoid' 'by' P ]" := [Setoid by P on _].
 
-  Notation "(== 'in' A )" := (setoid_equal A).
-  Notation "x == y 'in' A" := (setoid_equal A x y) (at level 70, y at next level, no associativity).
-  Notation "(==)" := (== in _).
-  Notation "x == y" := (x == y in _) (at level 70, no associativity).
+Notation "(== 'in' A )" := (setoid_equal A).
+Notation "x == y 'in' A" := (setoid_equal A x y) (at level 70, y at next level, no associativity).
+Notation "(==)" := (== in _).
+Notation "x == y" := (x == y in _) (at level 70, no associativity).
 
-  Program Definition eq_setoid (X:Type) :=
-    [Setoid by @eq X].
-  Program Definition function (X Y:Type) : Setoid :=
-    [Setoid by `(forall x, f x = g x) on X -> Y].
-  Next Obligation.
-    split; intros x; congruence.
-  Defined.
-  (* Canonical Structure function. *)
 
-  Inductive empty := .
+Program Definition eq_setoid (X:Type) :=
+  [Setoid by @eq X].
 
-  Program Definition empty_setoid: Setoid :=
-    [Setoid by (fun e e' => match e, e' with end) on empty].
-  Next Obligation.
-    split; compute; intros x; case x.
-  Qed.
+Program Definition function (X Y:Type) : Setoid :=
+  [Setoid by `(forall x, f x = g x) on X -> Y].
+Next Obligation.
+  split; intros x; congruence.
+Defined.
+Canonical Structure function.
 
-  Inductive unit := tt.
+Program Definition prop_setoid :=
+  [Setoid by iff].
+Canonical Structure prop_setoid.
+
+Inductive empty := .
+
+Program Definition empty_setoid: Setoid :=
+  [Setoid by (fun e e' => match e, e' with end) on empty].
+Next Obligation.
+  split; compute; intros x; case x.
+Qed.
+
+Inductive unit := tt.
+
+Program Definition unit_setoid: Setoid :=
+  [Setoid by (fun _ _ => True) on unit].
+Next Obligation.
+  split; intros H; tauto.
+Qed.
+
+
+Class IsSubSetoid (X:Setoid) (conf: X -> Prop) := 
+{ subconf_proper:> Proper ((==) ==> (==)) conf }.
+
+Structure SubSetoid (X:Setoid) := {
+  sub_conf:> X -> Prop;
+  sub_prf:> IsSubSetoid X sub_conf
+}.
+#[global]
+Existing Instance sub_prf.
+
+Notation "[ 'SubSetoid' 'by' conf 'on' A ]" :=
+  (@Build_SubSetoid A conf _).
+Notation "[ 'SubSetoid' 'by' conf ]" :=
+  [SubSetoid by conf on _].
+Notation "[ 'SubSetoid' 'of' x 'in' A | P ]" :=
+  [SubSetoid by (fun x => P) on A].
+Notation "[ 'SubSetoid' 'of' x | P ]" :=
+  [SubSetoid of x in _ | P].
+Program Definition subsetoid_as_setoid {A:Setoid} (B: SubSetoid A) :=
+  [Setoid by (== in A) on {x|B x}].
+Next Obligation.
+  split.
+  - now intros x.
+  - intros x y Heq. now symmetry.
+  - intros x y z Heq1 Heq2. now rewrite Heq1.
+Defined.
+Coercion subsetoid_as_setoid : SubSetoid >-> Setoid.
+
+Class IsMap {X Y:Setoid} (f: X -> Y) :=
+{ map_proper:> Proper ((==) ==> (==)) f }.
+
+Structure Map (X Y:Setoid): Type := {
+  map_fun:> X -> Y;
+  map_prf:> IsMap map_fun
+}.
+#[global]
+Existing Instance map_prf.
+
+Notation "[ 'Map' 'by' f ]" := (@Build_Map _ _ f _) : setoid_scope.
+Notation " 'map' x 'in' X => m " := [Map by fun (x:X) => m] (at level 70, right associativity) : setoid_scope.
+Notation " 'map' x => m " := (map x in _ => m) (at level 70, right associativity) : setoid_scope.
+
+Program Definition Map_compose {X Y Z:Setoid} (f: Map X Y) (g: Map Y Z)
+  : Map X Z := map x => g (f x).
+Next Obligation.
+  split. intros x y Heq. now rewrite Heq.
+Defined.
+
+Program Definition Map_id (X:Setoid) : Map X X := map x => x.
+Next Obligation.
+  split. intros x y Heq. apply Heq.
+Defined.
+
+Program Definition Map_setoid (X Y: Setoid) : Setoid :=
+  [Setoid by ((==) ==> (==))%signature on Map X Y].
+Next Obligation.
+  split.
+  - intros f x y Heq. now rewrite Heq. 
+  - intros f g Heq1 x y Heq2. now rewrite (Heq1 y x (symmetry Heq2)).
+  - intros f g h Heq1 Heq2 x y Heq3. 
+    now rewrite (Heq1 x y Heq3), <-(Heq2 x y Heq3), Heq3.
+Defined.
+Canonical Structure Map_setoid.
+
+Notation "g \o f" := (Map_compose f g) (at level 60, right associativity) : setoid_scope.
+
+Class Injective `(f: Map X Y) : Prop :=
+{ injective: forall x y, f x == f y -> x == y }.
+
+Class Surjective `(f: Map X Y) : Prop :=
+{ surjective: forall y, exists x, y == f x }.
+
+Class Bijective `(f: Map X Y) : Prop := {
+  bij_injective:> Injective f;
+  bij_surjective:> Surjective f
+}.
+
+Lemma mapcomp_reduc : forall {X Y Z} {f g: Map Y Z} {h: Map X Y},
+  Surjective h -> f \o h == g \o h -> f == g.
+Proof.
+  intros X Y Z f g h [Sh] Heq. simpl. intros x y Heq1.
+  rewrite Heq1. destruct (Sh y) as [x0 Heq2].
+  rewrite Heq2. now apply Heq.
+Qed.
+
+Lemma mapcomp_assoc : forall {X Y Z W} {f: Map Z W} {g: Map Y Z} {h: Map X Y},
+  (f \o g) \o h == f \o g \o h.
+Proof.
+  intros. simpl. intros x y Heq. now rewrite Heq.
+Qed.
+
+
+Declare Scope alg_scope.
+Open Scope alg_scope.
+
+Class IsBinop (X:Setoid) (op: X -> X -> X) :=
+{ binop_proper:> Proper ((==) ==> (==) ==> (==)) op }.
+
+Structure Binop (X:Setoid) := {
+  binop_op:> X -> X -> X;
   
-  Program Definition unit_setoid: Setoid :=
-    [Setoid by (fun _ _ => True) on unit].
-  Next Obligation.
-    split; intros H; tauto.
-  Qed.
+  binop_prf:> IsBinop X binop_op
+}.
+#[global]
+Existing Instance binop_prf.
 
-  Class IsMap {X Y:Setoid} (f: X -> Y) :=
-  { map_proper:> Proper ((==) ==> (==)) f }.
-  (* Print "==>".
-  Locate respectful. *)
+Notation "[ 'Binop' 'by' f ]" := (@Build_Binop _ f _) : alg_scope.
+Notation " 'binop' x , y 'in' A => m " := [Binop by fun (x y:A) => m] (at level 70, right associativity) : alg_scope.
+Notation " 'binop' x , y => m " := [Binop by fun (x y:_) => m] (at level 70, right associativity) : alg_scope.
 
-  Structure Map (X Y:Setoid): Type := {
-    map_fun:> X -> Y;
-    map_prf:> IsMap map_fun
-  }.
-  #[global]
-  Existing Instance map_prf.
-  
-  Notation "[ 'Map' 'by' f ]" := (@Build_Map _ _ f _).
-  Notation "[ x 'in' X :-> m ]" := [Map by fun (x:X) => m].
-  Notation "[ x :-> m ]" := ([x in _ :-> m]).
+Class Associative `(op: Binop X) := {
+  associative: 
+    forall x y z, op x (op y z) == op (op x y) z 
+}.
 
-  Program Definition Map_compose {X Y Z:Setoid} (f: Map X Y) (g: Map Y Z): Map X Z :=
-    [x :-> g (f x)].
-  Next Obligation.
-    split. intros x y Heq. now rewrite Heq.
-  Defined.
+Class LIdentical `(op: Binop X) (e:X) :=
+{ lidentical: forall x, op e x == x }.
 
-  Program Definition Map_id (X:Setoid) : Map X X :=
-    [x :-> x].
-  Next Obligation.
-    split. intros x y Heq. apply Heq.
-  Defined.
+Class RIdentical `(op: Binop X) (e:X) :=
+{ ridentical: forall x, op x e == x }.
 
-  Program Definition Map_setoid (X Y: Setoid) : Setoid :=
-    [Setoid by `(forall x, f x == g x) on Map X Y].
-  Next Obligation.
-    split.
-    - now intros x x0.
-    - intros x y Heq x0. now rewrite Heq.
-    - intros x y z Heq1 Heq2 x0. now rewrite Heq1, Heq2.
-  Defined.
-  Canonical Structure Map_setoid.
+Class Identical `(op: Binop X) (e:X) := {
+  identical_l:> LIdentical op e;
+  identical_r:> RIdentical op e
+}.
+#[global]
+Existing Instances identical_l identical_r.
 
-  (* Program Definition Map_setoid' (X Y:Setoid) : Setoid :=
-    [Setoid by ((==)==>(==))%signature on Map X Y]. *)
+Class LInvertible `(op: Binop X) (e:X) (inv: Map X X) :=
+{ linvertible: forall x, op (inv x) x == e }.
 
-  Definition injective `(f: Map X Y) :=
-    forall x y, f x == f y -> x == y.
-  Definition surjective `(f: Map X Y) :=
-    forall y, exists x, y == f x.
-  Definition bijective `(f: Map X Y) :=
-    injective f /\ surjective f.
-End Setoid.
-Import Setoid.
+Class RInvertible `(op: Binop X) (e:X) (inv: Map X X) :=
+{ rinvertible: forall x, op x (inv x) == e }.
 
-Declare Scope group_scope.
-Open Scope group_scope.
-Module Group.
-  Class IsGroup 
-        (supp:Setoid)
-        (op: supp -> supp -> supp)
-        (inv: Map supp supp)
-        (id:supp) := 
-  {
-    grp_op_proper:>
-      Proper ((==) ==> (==) ==> (==)) op;
-    
-    grp_op_assoc:
-      forall {x y z}, op x (op y z) == op (op x y) z;
-    
-    grp_inv_l:
-      forall {x}, op (inv x) x == id;
-    grp_inv_r:
-      forall {x}, op x (inv x) == id;
-    
-    grp_id_r:
-      forall {x}, op x id == x
-  }.
+Class Invertible `{Identical X op e} (inv: Map X X) := {
+  invertible_l:> LInvertible op e inv;
+  invertible_r:> RInvertible op e inv
+}.
+#[global]
+Existing Instances invertible_l invertible_r.
 
-  Structure Group :=
-  {
-    grp_supp:> Setoid;
-    grp_op: grp_supp -> grp_supp -> grp_supp;
-    grp_inv: Map grp_supp grp_supp;
-    grp_id:grp_supp;
 
-    grp_prf:> IsGroup grp_supp grp_op grp_inv grp_id
-  }.
-  #[global]
-  Existing Instance grp_prf.
+Class IsGroup 
+      (supp:Setoid)
+      (op: Binop supp)
+      (inv: Map supp supp)
+      (e:supp) := 
+{
+  grp_op_assoc:> Associative op;
+  grp_id_ident_r:> RIdentical op e;
+  grp_inv_invert_r:> RInvertible op e inv
+}.
 
-  Notation "[ 'Group' 'by' op , inv , id 'on' A ]" :=
-    (@Build_Group A op inv id _).
-  Notation "[ 'Group' 'by' op , inv , id ]" :=
-    [Group by op, inv, id on _].
-  
-  Notation "g *_{ G } h" := (@grp_op G g h) (at level 60, right associativity) : group_scope.
-  Notation "g * h" := (g *_{_} h) : group_scope.
-  Notation "id_{ G }" := (@grp_id G) : group_scope.
-  Notation "'id'" := id_{_} : group_scope.
-  Notation "!_{ G } g " := (@grp_inv G g) (at level 30, right associativity) : group_scope.
-  Notation "! g" := (!_{_} g) (at level 30, right associativity): group_scope.
-End Group.
-Import Group.
+Structure Group :=
+{
+  grp_supp:> Setoid;
+  grp_op: Binop grp_supp;
+  grp_inv: Map grp_supp grp_supp;
+  grp_id: grp_supp;
+
+  grp_prf:> IsGroup grp_supp grp_op grp_inv grp_id
+}.
+#[global]
+Existing Instance grp_prf.
+
+Notation "[ 'group' 'by' op , inv , id 'on' A ]" :=
+  (@Build_Group A op inv id _).
+Notation "[ 'group' 'by' op , inv , id ]" :=
+  [group by op, inv, id on _].
+
+Notation "( * 'in' G )" := (@grp_op G) : alg_scope.
+Notation "( * )" := ( * in _) : alg_scope.
+Notation "g *_{ G } h" := (@grp_op G g h) (at level 60, right associativity) : alg_scope.
+Notation "g * h" := (g *_{_} h) : alg_scope.
+Notation "1_{ G }" := (@grp_id G) : alg_scope.
+Notation "'1'" := 1_{_} : alg_scope.
+Notation "(\! 'in' G ) " := (@grp_inv G) : alg_scope.
+Notation "(\!)" := (\! in _) : alg_scope.
+Notation "!_{ G } g " := (@grp_inv G g) (at level 30, right associativity) : alg_scope.
+Notation "! g" := ( !_{_} g) (at level 30, right associativity): alg_scope.
+
+Lemma grp_id_ident_l : forall {G:Group}, LIdentical ( * in G) 1.
+Proof.
+  split. intros x.
+  assert (1 * x == 1 * (x * 1)) as Heq0. { now rewrite ridentical. }
+  assert (x * 1 == x * !x * !!x) as Heq1.
+  { now rewrite <-(rinvertible (!x)), associative. }
+  rewrite Heq0, Heq1, rinvertible, associative, ridentical.
+  assert (1 == x * !x) as Heq2. { now rewrite rinvertible. }
+  now rewrite Heq2, <-associative, rinvertible, ridentical.
+Qed.
+#[global]
+Existing Instance grp_id_ident_l.
+
+Lemma grp_inv_invert_l : forall {G:Group}, LInvertible ( * in G) 1 (\!).
+Proof.
+  split. intros x.
+  assert (!x * x == !x * (x * !x) * !!x) as Heq0.
+  { now rewrite associative, <-associative, rinvertible, ridentical. }
+  now rewrite Heq0, rinvertible, ridentical, rinvertible.
+Qed.
+#[global]
+Existing Instance grp_inv_invert_l.
 
 Section GroupTheory.
   Context {G:Group}.
-  Lemma grp_id_l : forall {x:G}, id * x == x.
-  Proof.
-    intros x. 
-    now rewrite <-(grp_inv_r(x:=x)),
-      <-grp_op_assoc, (grp_inv_l), grp_id_r.
-  Qed.
-
-  Lemma grp_op_inj_l : forall {g x y:G},
-    g * x == g * y -> x == y.
-  Proof.
-    intros g x y Heq.
-    assert (!g * g * x == !g * g * y) as H.
-    { now rewrite <-2!grp_op_assoc, Heq. }
-    now rewrite grp_inv_l, 2!grp_id_l in H.
-  Qed.
-
   Lemma grp_op_inj_r : forall {g x y:G},
     x * g == y * g -> x == y.
   Proof.
     intros g x y Heq.
     assert (x * (g * !g) == y * (g * !g)) as H.
-    { now rewrite 2!grp_op_assoc, Heq. }
-    now rewrite grp_inv_r, 2!grp_id_r in H.
+    { now rewrite 2!associative, Heq. }
+    now rewrite rinvertible, 2!ridentical in H.
+  Qed.
+
+  Lemma grp_op_inj_l : forall {g x y:G},
+    g * x == g * y -> x == y.
+  Proof.
+    intros g x y Heq. 
+    assert (!g * g * x == !g * g * y) as H.
+    { now rewrite <-2!associative, Heq. }
+    now rewrite linvertible, 2!lidentical in H.
   Qed.
 
   Lemma grp_op_feq_l : forall {g x y:G},
@@ -189,7 +293,7 @@ Section GroupTheory.
   Proof.
     intros g x y Heq.
     apply (grp_op_inj_l(g:=g)).
-    now rewrite grp_op_assoc, grp_inv_r, grp_id_l.
+    now rewrite associative, rinvertible, lidentical.
   Qed.
 
   Lemma grp_send_r : forall {g x y:G},
@@ -197,14 +301,14 @@ Section GroupTheory.
   Proof.
     intros g x y Heq.
     apply (grp_op_inj_r(g:=g)).
-    now rewrite <-grp_op_assoc, grp_inv_l, grp_id_r.
+    now rewrite <-associative, linvertible, ridentical.
   Qed.
   
   Lemma grp_invinv : forall {x:G}, !!x == x.
   Proof.
     intros x.
     assert (!!x * !x == x * !x) as H.
-    { now rewrite grp_inv_l, grp_inv_r. }
+    { now rewrite linvertible, rinvertible. }
     now apply grp_op_inj_r in H.
   Qed.
 
@@ -212,331 +316,302 @@ Section GroupTheory.
     !(x * y) == !y * !x.
   Proof.
     intros x y. 
-    rewrite <-(grp_id_r(x:=!y*!x)), <-grp_op_assoc.
+    rewrite <-(ridentical (!y * !x)), <-associative.
     apply grp_send_l, grp_send_l.
-    now rewrite grp_op_assoc, grp_inv_r.
+    now rewrite associative, rinvertible.
   Qed.
 
-  Lemma grp_invid_id : !id_{G} == id.
+  Lemma grp_invid_id : !1_{G} == 1.
   Proof.
-    rewrite <-(grp_id_r(x:=!id)).
-    symmetry; apply grp_send_l, grp_id_l.
+    rewrite <-(ridentical (!1)).
+    symmetry; apply grp_send_l, lidentical.
   Qed.
 End GroupTheory.
 
-Module Hom.
-  Class IsHom {G H:Group} (f: Map G H) := {
-    hom_proper:
-      forall {x y:G}, f (x * y) == (f x) * (f y)
-  }.
 
-  Structure Hom (G H:Group) := {
-    hom_map:> Map G H;
-    
-    hom_prf:> IsHom hom_map
-  }.
-  #[global]
-  Existing Instance hom_prf.
+Class IsHomomorph {G H:Group} (f: Map G H) := {
+  homomorph:
+    forall {x y:G}, f (x * y) == (f x) * (f y)
+}.
 
-  Notation "[ 'Hom' 'by' f ]" := (@Build_Hom _ _ [Map by f] _) : group_scope.
-  Notation "[ x 'in' G :-> m ]" := [Hom by fun (x:G) => m] : group_scope.
-  Notation "[ x :-> m ]" := ([x in _ :-> m]) : group_scope.
+Structure Homomorph (G H:Group) := {
+  hom_map:> Map G H;
+  
+  hom_prf:> IsHomomorph hom_map
+}.
+#[global]
+Existing Instance hom_prf.
 
-  Class IsIsomorph `(f: Hom G H) := {
-    iso_proper: bijective f
-  }.
+Notation "[ 'Hom' 'by' f ]" := (@Build_Homomorph _ _ [Map by f] _) : alg_scope.
+Notation " 'hom' x 'in' G => m " := [Hom by fun (x:G) => m] (at level 70, right associativity) : alg_scope.
+Notation " 'hom' x => m " := (hom x in _ => m) (at level 70, right associativity) : alg_scope.
 
-  Structure Isomorph (G H:Group):= {
-    iso_map:> Hom G H;
+Class IsIsomorph `(f: Homomorph G H) := {
+  isomorph:> Bijective f
+}.
 
-    iso_prf:> IsIsomorph iso_map
-  }.
-  #[global]
-  Existing Instance iso_prf.
-  Notation "[ 'Iso' 'by' f ]" := (@Build_Isomorph _ _ [Hom by f] _) : group_scope.
-  Notation "[ x 'in' G :=> m ]" := [Iso by fun (x:G) => m] : group_scope.
-  Notation "[ x :=> m ]" := ([x in _ :=> m]) : group_scope.
-End Hom.
-Import Hom.
+Structure Isomorph (G H:Group):= {
+  iso_map:> Homomorph G H;
+
+  iso_prf:> IsIsomorph iso_map
+}.
+#[global]
+Existing Instance iso_prf.
+Notation "[ 'Iso' 'by' f ]" := (@Build_Isomorph _ _ [Hom by f] _) : alg_scope.
+Notation "'iso' x 'in' G => m " := [Iso by fun (x:G) => m] (at level 70, right associativity) : alg_scope.
+Notation "'iso' x => m " := (iso x in _ => m) (at level 70, right associativity) : alg_scope.
+
 
 Section HomTheory.
-  Context {G H:Group} {f: Hom G H}.
-  Lemma hom_id : f id == id.
+  Context {G H:Group} {f: Homomorph G H}.
+  Lemma hom_id : f 1 == 1.
   Proof.
-    rewrite <-(grp_inv_r(x:=f id)).
-    apply grp_send_r. now rewrite <-hom_proper, grp_id_r.
+    rewrite <-(rinvertible (f 1)).
+    apply grp_send_r. now rewrite <-homomorph, ridentical.
   Qed.
 
   Lemma hom_inv : forall x, f (!x) == ! f x.
   Proof.
     intros x.
-    rewrite <-(grp_id_r(x:=!f x)).
+    rewrite <-(ridentical (!(f x))).
     apply grp_send_l.
-    now rewrite <-hom_proper, grp_inv_r, hom_id.
+    now rewrite <-homomorph, rinvertible, hom_id.
   Qed.
 End HomTheory.
 
-Module SubGroup.
-  Class IsSubGroup (G:Group) (H: G -> Prop) :=
-  {
-    sg_conf_proper:
-      forall {x y}, x == y -> H x -> H y;
 
-    sg_ferm_op:
-      forall {x y}, H x -> H y -> H (x * y);
-    
-    sg_ferm_inv:
-      forall {x}, H x -> H (!x);
-    
-    sg_ferm_id: H id
-  }.
-
-  Structure SubGroup := {
-    sg_G: Group;
-    sg_H:> sg_G -> Prop;
-
-    sg_prf:> IsSubGroup sg_G sg_H
-  }.
-  #[global]
-  Existing Instance sg_prf.
+Class IsSubGroup (G:Group) (H: SubSetoid G) :=
+{
+  sg_ferm_op:
+    forall {x y}, H x -> H y -> H (x * y);
   
-  Notation "[ 'SubGroup' H 'on' G ]" :=
-    (@Build_SubGroup G H _).
-  Notation "[ 'SubGroup' 'of' x : G | P ]" :=
-    [SubGroup (fun x => P) on G].
-  Notation "[ 'SubGroup' 'of' x | P ]" :=
-    [SubGroup (fun x => P) on _].
+  sg_ferm_inv:
+    forall {x}, H x -> H (!x);
+  
+  sg_ferm_id: H 1
+}.
 
-  Program Definition sg_as_setoid (H:SubGroup) :=
-    [Setoid by (fun x y => proj1_sig x == proj1_sig y) on {x|H x}].
-  Next Obligation.
-    split.
-    - now intros x.
-    - intros x y Heq. now symmetry.
-    - intros x y z Heq1 Heq2. now rewrite Heq1, Heq2.
-  Defined.
-  Coercion sg_as_setoid : SubGroup >-> Setoid.
+Structure SubGroup (G:Group) := {
+  sg_supp:> SubSetoid G;
 
-  Program Definition sg_as_group (H:SubGroup) :=
-    [Group by (fun x y => x * y),
-              [Map by fun x => !x], 
-              (id_{sg_G H}) on H].
-  Next Obligation.
-    apply sg_ferm_op; (apply H1 || apply H0).
-  Defined.
-  Next Obligation.
-    apply sg_ferm_inv, H0.
-  Defined.
-  Next Obligation.
-    split. intros x y. simpl. now intros Heq; rewrite Heq.
-  Defined.
-  Next Obligation.
+  sg_prf:> IsSubGroup G sg_supp
+}.
+#[global]
+Existing Instance sg_prf.
+
+Notation "H '<-' G" :=
+  (@Build_SubGroup G H _) (at level 60, right associativity) : alg_scope.
+Notation "[ 'subgroup' 'of' x 'in' G | P ] " :=
+  ([SubSetoid of x | P] <- G) : alg_scope.
+Notation "[ 'subgroup' 'of' x | P ]" :=
+  ([subgroup of x in _ | P]) : alg_scope.
+
+Program Definition sg_as_group `(H:SubGroup G) :=
+  [group by (binop x, y => x * y), (map x => !x), 1 on H].
+Next Obligation.
+  apply sg_ferm_op; (apply H1 || apply H0).
+Defined.
+Next Obligation.
+  split. intros x1 y1 Heq x0 y0 Heq1. simpl. 
+  simpl in Heq. simpl in Heq1. now rewrite Heq, Heq1.
+Defined.
+Next Obligation.
+  apply sg_ferm_inv, H0.
+Defined.
+Next Obligation.
+  split. intros x y. simpl. intros Heq.
+  now rewrite Heq.
+Defined.
+Next Obligation.
+  apply sg_ferm_id.
+Defined.
+Next Obligation.
+  split.
+  - split. intros x y z. simpl. apply associative.
+  - split. intros x. simpl. apply ridentical.
+  - split. intros x. simpl. apply rinvertible.
+Defined.
+Coercion sg_as_group : SubGroup >-> Group.
+
+Class IsNormalSubGroup `(H: SubGroup G) := {
+  normal:
+    forall {g h}, H h -> H (g * h * !g)
+}.
+
+Structure NormalSubGroup (G:Group):= {
+  nsg_supp:> SubGroup G;
+
+  nsg_prf:> IsNormalSubGroup nsg_supp
+}.
+#[global]
+Existing Instance nsg_prf.
+
+Notation "H <| G" :=
+  (@Build_NormalSubGroup G H _) (at level 60, right associativity) : alg_scope.
+
+
+Program Definition HomImage `(f: Homomorph G H):= 
+  [subgroup of y | exists x, y == f x].
+Next Obligation.
+  split.
+  - intros x y Heq. apply conj; 
+    intros [z Heq1]; exists z; now rewrite <-Heq1, Heq.
+Defined.
+Next Obligation.
+  split.
+  - intros x y. simpl. intros [z1 Heq1] [z2 Heq2].
+    exists (z1 * z2). now rewrite homomorph, Heq1, Heq2.
+  - intros x [y Heq].
+    exists (!y).
+    now rewrite hom_inv, Heq.
+  - exists 1. symmetry; apply hom_id.
+Defined.
+
+Program Definition confimg `(f: Homomorph G H) 
+  : Homomorph G (HomImage f) := hom g => f g.
+Next Obligation.
+  now exists g.
+Defined.
+Next Obligation.
+  split. intros x y Heq. simpl. now rewrite Heq.
+Defined.
+Next Obligation.
+  split. intros x y. simpl. apply homomorph.
+Defined.
+
+Lemma confimg_surj `{f: Homomorph G H} : Surjective (confimg f).
+Proof.
+  split. intros [h [g Heq]]. simpl. now exists g.
+Qed.
+#[global]
+Existing Instance confimg_surj.
+
+Program Definition inclusion `{f: Homomorph G H}
+  : Homomorph (HomImage f) H := hom h => h.
+Next Obligation. split. intros x y. now simpl. Defined.
+Next Obligation. split. intros x y. now simpl. Defined.
+
+Lemma inc_inj `{f: Homomorph G H} : Injective (@inclusion _ _ f).
+Proof. split. intros x y. now simpl. Qed.
+
+Program Definition HomKernel `(f: Homomorph G H) :=
+  [subgroup of x | f x == 1] <| G.
+Next Obligation.
+  split. intros g h. simpl. intros Heq. apply conj;
+  intros Heq1; now rewrite <-Heq1, Heq.
+Defined.
+Next Obligation.
+  split; simpl.
+  - intros x y Heq1 Heq2.
+    now rewrite homomorph, Heq1, Heq2, ridentical.
+  - intros x Heq.
+    now rewrite hom_inv, Heq, grp_invid_id.
+  - apply hom_id.
+Defined.
+Next Obligation.
+  split. simpl. intros g h Heq0.
+  now rewrite 2!homomorph, Heq0, ridentical,
+    <-homomorph, rinvertible, hom_id.
+Defined.
+
+
+Program Definition Coset `(H: SubGroup G) :=
+  [Setoid by (fun x y => H (x * !y)) on G].
+Next Obligation.
+  split.
+  - intros x. rewrite rinvertible. apply sg_ferm_id.
+  - intros x y Heq. apply sg_ferm_inv in Heq.
+    now rewrite grp_opinv, grp_invinv in Heq.
+  - intros x y z Hxy Hyz.
+    pose (sg_ferm_op Hxy Hyz) as Hxz.
+    now rewrite associative, <-(associative x (!y) y), 
+      linvertible, ridentical in Hxz.
+Defined.
+
+Program Definition quotmap `{H: SubGroup G} : Map G (Coset H) :=
+  map x => x.
+Next Obligation.
+  split. intros x y Heq. simpl. rewrite Heq, rinvertible.
+  apply sg_ferm_id.
+Defined.
+(* Coercion _quotmap `{H: SubGroup G} : G -> Coset H := quotmap. *)
+
+Lemma quotmap_surj `{H: SubGroup G} : Surjective (@quotmap G H).
+Proof.
+  split. intros g. simpl. exists g. rewrite rinvertible. apply sg_ferm_id.
+Defined.
+#[global]
+Existing Instance quotmap_surj.
+
+Program Definition CosetGroup `(H: NormalSubGroup G) :=
+  [group by (binop x, y => x * y), (map x => !x), 1 on Coset H].
+Next Obligation.
+  split. intros x0 y0. simpl. intros Heq0 x1 y1 Heq1.
+  assert (H (x0 * x1 * !y1 * !x0)) as Heq2.
+  { rewrite <-(associative _ _ (!y1)). now apply normal. }
+  pose (sg_ferm_op Heq2 Heq0) as Heq3.
+  rewrite associative, <-(associative _ (!x0) x0),
+    linvertible, ridentical in Heq3.
+  now rewrite grp_opinv, associative.
+Defined.
+Next Obligation.
+  split. intros x y. simpl. intros Heq. rewrite <-grp_opinv.
+  apply sg_ferm_inv. apply (normal(g := !y)) in Heq.
+  now rewrite grp_invinv, associative, <-(associative _ (!y) y),
+    linvertible, ridentical in Heq.
+Defined.
+Next Obligation.
+  split; split.
+  - intros x y z. simpl. rewrite associative, rinvertible.
     apply sg_ferm_id.
-  Defined.
-  Next Obligation.
-    split.
-    - intros x1 x2 Heq_x y1 y2 Heq_y. simpl.
-      apply grp_op_proper; (apply Heq_x || apply Heq_y).
-    - intros x y z. simpl. apply grp_op_assoc.
-    - intros x. simpl. apply grp_inv_l.
-    - intros x. simpl. apply grp_inv_r.
-    - intros x. simpl. apply grp_id_r.
-  Defined.
-  Coercion sg_as_group : SubGroup >-> Group.
-
-  Class IsNormalSG (H:SubGroup) := {
-    nsg_proper:
-      forall {g h}, H h -> H (g * h * !g)
-  }.
-
-  Structure NormalSG := {
-    nsg_H:> SubGroup;
-
-    nsg_prf:> IsNormalSG nsg_H
-  }.
-  #[global]
-  Existing Instance nsg_prf.
-
-  Notation "[ 'NSG' H 'on' G ]" :=
-    (@Build_NormalSG [SubGroup H on G] _).
-  Notation "[ 'NSG' 'of' x : G | P ]" :=
-    [NSG (fun x => P) on G].
-  Notation "[ 'NSG' 'of' x | P ]" :=
-    [NSG (fun x => P) on _].
-End SubGroup.
-Import SubGroup.
-
-Section HomTheory.
-  Context {G H:Group} (f: Hom G H).
-  Program Definition ImageSG := 
-    [SubGroup of y | exists x, y == f x].
-  Next Obligation.
-    split.
-    - intros x y Heq1 [z Heq2].
-      exists z. now rewrite <-Heq1.
-    - intros x y [z_x Heq1] [z_y Heq2].
-      exists (z_x * z_y).
-      now rewrite Heq1, Heq2, hom_proper.
-    - intros x [y Heq].
-      exists (!y).
-      now rewrite hom_inv, Heq.
-    - exists id. symmetry; apply hom_id.
-  Defined.
-  
-  Program Definition confimg : Hom G ImageSG :=
-    [g :-> f g].
-  Next Obligation.
-    now exists g.
-  Defined.
-  Next Obligation.
-    split. intros x y Heq. simpl. now rewrite Heq.
-  Defined.
-  Next Obligation.
-    split. intros x y. simpl. apply hom_proper.
-  Defined.
-  (* Canonical confimg. *)
-
-  Lemma confimg_surj : surjective confimg.
-  Proof.
-    intros [h [g Heq]]. simpl. now exists g.
-  Qed.
-
-  Program Definition inc : Hom ImageSG H :=
-    [h :-> h].
-  Next Obligation.
-    split. intros x y. now simpl.
-  Defined.
-  Next Obligation.
-    split. intros x y. now simpl.
-  Defined.
-
-  Lemma inc_inj : injective inc.
-  Proof.
-    intros x y. now simpl.
-  Qed.
-
-  Program Definition KernelNSG :=
-    [NSG of x | f x == id].
-  Next Obligation.
-    split.
-    - intros x y Heq1 Heq2. now rewrite <-Heq1. 
-    - intros x y Heq1 Heq2.
-      now rewrite hom_proper, Heq1, Heq2, grp_id_r.
-    - intros x Heq.
-      now rewrite hom_inv, Heq, grp_invid_id.
-    - apply hom_id.
-  Defined.
-  Next Obligation.
-    split. intros g h. simpl. intros Heq.
-    now rewrite 2!hom_proper, Heq, grp_id_r,
-      <-hom_proper, grp_inv_r, hom_id.
-  Defined.
-End HomTheory.
-
-Ltac Hrewrite Heq := apply (sg_conf_proper Heq).
-Ltac Hrewriteto x := apply (sg_conf_proper(x:=x)).
-
-Module Coset.
-  Program Definition Coset (H:SubGroup) :=
-    [Setoid by (fun x y => H (x * !y)) on (sg_G H)].
-  Next Obligation.
-    split.
-    - intros x. 
-      apply (sg_conf_proper (symmetry grp_inv_r)), sg_ferm_id.
-    - intros x y Heq.
-      apply (sg_conf_proper grp_invinv), sg_ferm_inv.
-      apply (sg_conf_proper (symmetry grp_opinv)).
-      now apply (sg_conf_proper(x:=x*!y)); (rewrite grp_invinv || idtac).
-    - intros x y z Hxy Hyz. 
-      apply (sg_conf_proper(x:=(x*!y)*(y*!z))).
-     -- now rewrite grp_op_assoc, <-(grp_op_assoc(x:=x)), 
-          grp_inv_l, grp_id_r.
-     -- apply sg_ferm_op; (apply Hxy || apply Hyz).
-  Defined.
-
-  Program Definition proj {H:SubGroup} : Map (sg_G H) (Coset H) :=
-    [Map by fun x => x].
-  Next Obligation.
-    split. intros x y Heq. simpl. Hrewriteto id_{sg_G H}.
-    - now rewrite Heq, grp_inv_r.
-    - apply sg_ferm_id.
-  Defined.
-
-  Program Definition CosetGroup (H:NormalSG) :=
-    [Group by (fun x y => x * y), [Map by fun x => !x], id
-    on Coset H].
-  Next Obligation.
-    split. intros x y. simpl. intros Heq. Hrewriteto (!(!y*x)).
-    - now rewrite <-grp_opinv.
-    - apply sg_ferm_inv. Hrewriteto (!y * (x * !y) * !!y).
-     -- now rewrite grp_invinv, grp_op_assoc,
-          <-(grp_op_assoc(y:=!y)), grp_inv_l, grp_id_r.
-     -- now apply nsg_proper.
-  Defined.
-  Next Obligation.
-    split.
-    - intros x1 y1. simpl. intros Heq1 x2 y2 Heq2.
-      Hrewriteto (x1 * (x2 * !y2) * !x1 * (x1 * !y1)).
-     -- rewrite grp_opinv, 3!grp_op_assoc.
-        apply grp_op_feq_r. 
-        now rewrite <-grp_op_assoc, grp_inv_l, grp_id_r.
-     -- apply (nsg_proper(g:=x1)) in Heq2. 
-        apply (sg_ferm_op Heq2 Heq1).
-    - intros x y z. simpl. Hrewriteto id_{sg_G H}.
-     -- now rewrite grp_op_assoc, grp_inv_r.
-     -- apply sg_ferm_id.
-    - intros x. simpl. Hrewriteto id_{sg_G H}.
-     -- now rewrite grp_inv_l, grp_id_l, grp_invid_id.
-     -- apply sg_ferm_id.
-    - intros x. simpl. Hrewriteto id_{sg_G H}.
-     -- now rewrite grp_inv_r, grp_id_l, grp_invid_id.
-     -- apply sg_ferm_id.
-    - intros x. simpl. apply nsg_proper, sg_ferm_id.
-  Defined.
-  
-End Coset.
-Import Coset.
+  - intros x. simpl. apply normal, sg_ferm_id.
+  - intros x. simpl. rewrite grp_invid_id, ridentical, rinvertible.
+    apply sg_ferm_id.
+Defined.
 
 Section FundHom.
-  Context {G H:Group} (f: Hom G H) (N := KernelNSG f)
-    (G_N := CosetGroup N).
-  
-  Program Definition psi : Isomorph G_N (ImageSG f):=
-    [x :=> f x].
+  Context {G H:Group} (f: Homomorph G H)
+    (N := HomKernel f) (G_N := CosetGroup N).
+
+  Program Definition Iso1 : Isomorph G_N (HomImage f):=
+    iso x => f x.
   Next Obligation.
     now exists x.
   Defined.
   Next Obligation.
     split. intros x y. simpl. intros Heq.
-    rewrite hom_proper, hom_inv in Heq.
+    rewrite homomorph, hom_inv in Heq.
     apply grp_send_r in Heq.
-    now rewrite grp_invinv, grp_id_l in Heq.
+    now rewrite grp_invinv, lidentical in Heq.
   Defined.
   Next Obligation.
-    split. intros x y. simpl. apply hom_proper.
+    split. intros x y. simpl. apply homomorph.
   Defined.
   Next Obligation.
-    split. apply conj.
+    split; split; split.
     - intros x y. simpl. intros Heq.
-      rewrite hom_proper, hom_inv.
+      rewrite homomorph, hom_inv.
       symmetry; apply grp_send_r.
-      now rewrite grp_id_l.
+      now rewrite lidentical.
     - intros [y [x Heq]]. simpl. now exists x.
   Defined.
 
-  Lemma psicomp_proper :
-    f == Map_compose proj (Map_compose psi (inc _)) in (Map_setoid G H).
-  Proof.
-    intros g. now simpl.
-  Qed.
+  Lemma Iso1comp_proper :
+    f == inclusion \o Iso1 \o quotmap in (Map_setoid G H).
+  Proof. intros x y Heq. simpl. now rewrite Heq. Qed.
 
-  Lemma psi_identified : forall (psi0: Hom G_N H), 
-    f == Map_compose proj psi0 in (Map_setoid G H) ->
-    psi0 == Map_compose psi (inc _) in (Map_setoid G_N H).
+  Lemma Iso1_identified : forall (psi: Homomorph G_N H), 
+    f == psi \o quotmap in (Map_setoid G H) ->
+    psi == inclusion \o Iso1 in (Map_setoid G_N H).
   Proof.
-    simpl. now intros psi0 Hiso g.
+    intros psi Hiso x y Heq. rewrite Heq.
+    rewrite Iso1comp_proper in Hiso.
+    rewrite <-mapcomp_assoc in Hiso.
+    pose (mapcomp_reduc _ Hiso) as Heq2.
+    symmetry. now apply Heq2.
   Qed.
 End FundHom.
 
-Close Scope group_scope.
+Close Scope alg_scope.
+Close Scope setoid_scope.
 
